done/Iron/Language/SystemF2Data/Exp/Lit.v
@@ -1,9 +1,17 @@
 
+Require Import Iron.Language.SystemF2Data.Type.
+
 
 Inductive lit : Type :=
  (* Literal natural number. *)
  | LNat   : nat  -> lit
 
  (* Literal boolean. *)
- | Bool   : bool -> lit.
+ | LBool  : bool -> lit.
 
+
+Fixpoint typeOfLit (l : lit) : ty := 
+ match l with
+ | LNat  _   => TCon TyConNat
+ | LBool _   => TCon TyConBool
+ end.
